---
title: "指数函数求导证明"
date: "2019-03-08"
categories: 
  - "数学"
---

\\\[\\begin{align\*}\\\\ 设指数函数y&=a^x\\\\ y'&=\\underset{\\Delta x\\rightarrow 0}{lim}\\left\[\\frac{a^{\\left(x+\\Delta x\\right)}-a^x}{\\Delta x}\\right\]\\\\ &=\\underset{\\Delta x\\rightarrow 0}{lim}\\left\[\\frac{a^x(a^{\\Delta x}-1)}{\\Delta x}\\right\]\\\\ &=\\underset{\\Delta x\\rightarrow 0}{lim}a^x\\left\[\\frac{(a^{\\Delta x}-1)}{\\Delta x}\\right\]\\\\ &=a^x\\underset{\\Delta x\\rightarrow 0}{lim}\\left\[\\frac{(a^{\\Delta x}-1)}{\\Delta x}\\right\]\\\\ 设\\beta&=a^{\\Delta x}-1\\\\ 则a^{\\Delta x}&=1+\\beta\\\\ \\Delta x&=log\_a^{\\left(1+\\beta\\right)}\\\\ 因此：&\\\\ \\left\[\\frac{(a^{\\Delta x}-1)}{\\Delta x}\\right\]&=\\frac{\\beta}{log\_a^{\\left(1+\\beta\\right)}}\\\\ &=\\frac{1}{log\_a^{\\left(1+\\beta\\right)^{\\frac{1}{\\beta}}}}\\\\ &已知自然对数是：当n趋向无穷大时，\\underset{n\\rightarrow\\infty}{lim}\\left(1+\\frac{1}{n}\\right)^{n}=e\\\\ &当\\Delta x\\rightarrow 0 时， \\beta\\rightarrow 0 ，而这个\\beta正好可以比作n，\\\\ &也就是说\\left(1+\\beta\\right)^{\\frac{1}{\\beta}}=e\\\\ 故：&\\\\ \\underset{\\Delta x\\rightarrow 0}{lim}\\left\[\\frac{(a^{\\Delta x}-1)}{\\Delta x}\\right\]&=\\underset{\\beta\\rightarrow 0}{lim}\\frac{1}{log\_a^{\\left(1+\\beta\\right)^{\\frac{1}{\\beta}}}}\\\\ &=\\frac{1}{log\_a e}\\\\ &=ln a\\\\ 再次带入求导公式&\\\\ y'&=a^x\\underset{\\Delta x\\rightarrow 0}{lim}\\left\[\\frac{(a^{\\Delta x}-1)}{\\Delta x}\\right\]\\\\ &=a^x ln a \\end{align\*}\\\\\\\]
